wip: refactoring eo_fin proof

fairness/lawyer/examples/eo_fin/eo_fin.v
@@ -14,6 +14,314 @@ Definition EODegree n := bounded_nat n.
 Definition EOLevel n := bounded_nat n.
 
 
+Section SignalMap.
+
+  Class SigMapPreG Σ := {
+      sm_sig_map :> inG Σ (authUR (gmapUR nat (agreeR SignalId)));
+  }.
+  
+  Class SigMapG Σ := {
+      sm_PreG :> SigMapPreG Σ;
+      sm_γ__smap: gname;
+  }.
+
+  Context `{SigMapG Σ}.
+
+  Context `{DISCR__d: OfeDiscrete DegO} `{DISCR__l: OfeDiscrete LevelO}.
+  Context {LEQUIV__l: @LeibnizEquiv (ofe_car LevelO) (ofe_equiv LevelO)}.   
+  Let Degree := ofe_car DegO.
+  Let Level := ofe_car LevelO.
+  (* Context `{OP: ObligationsParams Degree Level Locale LIM_STEPS}. *)
+  Context `{OP': ObligationsParamsPre Degree Level LIM_STEPS}.
+  Let EO_OP := LocaleOP (Locale := locale heap_lang). 
+  Existing Instance EO_OP. 
+
+  Context {oGS: ObligationsGS Σ}.
+
+  Context (L: nat -> Level). 
+
+  Definition ex_ith_sig B (i: nat) (s: SignalId): iProp Σ :=
+    sgn s (L i) (Some $ B i) (oGS := oGS). 
+  
+  Definition smap_repr B K (smap: gmap nat SignalId): iProp Σ :=
+    own sm_γ__smap (● (to_agree <$> smap: gmapUR nat (agreeR SignalId))) ∗
+    ⌜ dom smap = set_seq 0 K ⌝ ∗
+    ([∗ map] i ↦ s ∈ smap, ex_ith_sig B i s).
+
+  Definition ith_sig (i: nat) (s: SignalId): iProp Σ :=
+    own sm_γ__smap (◯ {[ i := to_agree s ]}).
+
+  Lemma ith_sig_in i s B K (smap: gmap nat SignalId):
+    ⊢ ith_sig i s -∗ smap_repr B K smap -∗ ⌜ smap !! i = Some s ⌝.
+  Proof using.
+    iIntros "S (SM & ? & ?)". iCombine "SM S" as "SM".
+    iDestruct (own_valid with "SM") as %V.
+    apply auth_both_valid_discrete in V as [V ?].
+    apply singleton_included_l in V. destruct V as (x & ITH & LE).
+    iPureIntro.
+    rewrite Some_included_total in LE.
+    destruct (to_agree_uninj x) as [y X].
+    { eapply lookup_valid_Some; eauto. done. }
+    rewrite -X in LE. apply to_agree_included in LE.
+    rewrite -X in ITH.
+    
+    eapply leibniz_equiv.       
+    rewrite lookup_fmap in ITH.
+    rewrite -LE in ITH.
+    
+    apply fmap_Some_equiv in ITH as (?&ITH&EQ).
+    rewrite ITH. apply to_agree_inj in EQ. by rewrite EQ.
+  Qed.
+
+  Lemma ith_sig_sgn i s B K (smap: gmap nat SignalId):
+    ⊢ ith_sig i s -∗ smap_repr B K smap -∗ sgn s (L i) None (oGS := oGS).
+  Proof using.
+    iIntros "S SR".
+    iDestruct (ith_sig_in with "[$] [$]") as "%ITH". 
+    iDestruct "SR" as "(SM & % & ?)".
+    iDestruct (big_sepM_lookup with "[$]") as "ITH"; eauto.
+    rewrite /ex_ith_sig.     
+    by iDestruct (sgn_get_ex with "[$]") as "[??]". 
+  Qed.
+
+  Lemma smap_repr_split B K smap i s:
+    ⊢ ith_sig i s -∗ smap_repr B K smap -∗
+      ex_ith_sig B i s ∗ (ex_ith_sig B i s -∗ smap_repr B K smap).
+  Proof using.
+    iIntros "#ITH SR".
+    iDestruct (ith_sig_in with "[$] [$]") as "%ITH".
+    rewrite /smap_repr. iDestruct "SR" as "(SM & % & SR)".
+    rewrite {2 5}(map_split smap i) ITH /=.
+    rewrite !big_sepM_union.
+    2: apply map_disjoint_singleton_l_2; by apply lookup_delete.
+    iDestruct "SR" as "[S SR]". rewrite big_sepM_singleton.
+    iFrame. iIntros. iFrame. done.
+  Qed.
+
+  Lemma smap_repr_split_upd B B' m smap i s
+    (OTHER_PRES: forall j, j ≠ i -> j ∈ dom smap -> B' j = B j):
+    ⊢ ith_sig i s -∗ smap_repr B m smap -∗
+      ex_ith_sig B i s ∗ (ex_ith_sig B' i s -∗ smap_repr B' m smap).
+  Proof using LEQUIV__l DISCR__l DISCR__d.
+    iIntros "#ITH SR".
+    iDestruct (ith_sig_in with "[$] [$]") as "%ITH".
+    rewrite /smap_repr. iDestruct "SR" as "(SM & % & SR)".
+    rewrite {2 5}(map_split smap i) ITH /=.
+    rewrite !big_sepM_union.
+    2: apply map_disjoint_singleton_l_2; by apply lookup_delete.
+    iDestruct "SR" as "[S SR]". rewrite !big_sepM_singleton.
+    iFrame.
+    2: { apply map_disjoint_dom. set_solver. }
+    iIntros. iSplitR; [done| ]. iFrame.
+    iApply (big_sepM_impl with "[$]"). iIntros "!> %% %OTHER".
+    apply lookup_delete_Some in OTHER as [? ?%mk_is_Some%elem_of_dom]. 
+    rewrite /ex_ith_sig. rewrite OTHER_PRES; [by iIntros; iFrame| ..]; done. 
+  Qed.
+
+  (* TODO: use bupd in definition of OU *)
+  Lemma smap_create_ep i B K smap π π__cp τ d__h d__l
+    (PH_LE: phase_le π__cp π)
+    (LT: i < K)
+    (DEG_LT: deg_lt d__l d__h):
+    ⊢ smap_repr B K smap -∗ 
+      cp π__cp d__h (oGS := oGS) -∗
+      th_phase_ge τ π (oGS := oGS) -∗
+      |==> OU (∃ s, ith_sig i s ∗
+                    ep s π__cp d__l (oGS := oGS) ∗ smap_repr B K smap ∗
+                    th_phase_ge τ π (oGS := oGS)) (oGS := oGS).
+  Proof using DISCR__d DISCR__l LEQUIV__l.
+    iIntros "SR CP PH".
+    rewrite /smap_repr. iDestruct "SR" as "(AUTH & %DOM & SIGS)".
+    assert (i ∈ dom smap) as [s ITH]%elem_of_dom.
+    { rewrite DOM. apply elem_of_set_seq. lia. }
+    rewrite {2 5}(map_split smap i) ITH /=.
+    setoid_rewrite big_sepM_union.
+    2, 3: apply map_disjoint_singleton_l_2; by apply lookup_delete.
+    iDestruct "SIGS" as "[SIG SIGS]". setoid_rewrite big_sepM_singleton.
+    rewrite {1}/ex_ith_sig. 
+    iDestruct (create_ep_upd with "CP [$] [PH]") as "OU".
+    { eauto. }
+    { done. }
+    { done. }
+    iMod (own_update with "AUTH") as "X". 
+    { apply auth_update_dfrac_alloc. 
+      2: { apply singleton_included_l with (i := i).
+           rewrite lookup_fmap ITH. eexists. split; [| reflexivity].
+           simpl. reflexivity. }
+      apply _. }
+    iApply (OU_wand with "[-OU]"); [| by iFrame].
+    iIntros "(EP & SIG & PH)".
+    iDestruct "X" as "[? ITH]". 
+    iExists _. iFrame. done.
+  Qed.
+
+  (* TODO: move, find existing? *)
+  Lemma lookup_delete_ne' `{Countable K} {V: Type} (k: K) (m: gmap K V)
+    (NOk: k ∉ dom m):
+    delete k m = m.
+  Proof using.
+    apply map_eq. intros.
+    destruct (decide (i = k)) as [-> | ?].
+    - rewrite lookup_delete. symmetry.
+      by apply not_elem_of_dom.
+    - by apply lookup_delete_ne.
+  Qed.                          
+
+  Lemma smap_sgns_extend (B0: nat -> nat -> bool)
+    (smap: gmap nat SignalId) (s : SignalId) (m : nat) (* lm *)
+    (DOM: dom smap = set_seq 0 m)
+    (PRES: forall i, i ∈ dom smap -> B0 (m + 1) i = B0 m i)
+    (* (LVL: lvl2nat lm = m) *)
+    :
+    ⊢ ([∗ map] k↦y ∈ smap, sgn y (L k) (Some (B0 m k)) (oGS := oGS)) -∗
+       sgn s (L m) (Some (B0 (m + 1) m)) (oGS := oGS) -∗
+       [∗ map] i↦s0 ∈ <[m := s]> smap, sgn s0 (L i) (Some $ B0 (m + 1) i) (oGS := oGS).
+  Proof using.
+    iIntros "SIGS SG".
+    rewrite big_opM_insert_delete. 
+    iSplitL "SG"; [done| ].
+    rewrite lookup_delete_ne'.
+    2: { rewrite DOM. intros ?%elem_of_set_seq. lia. }
+    iApply (big_sepM_impl with "[$]"). iModIntro.
+    iIntros (??) "% ?".
+    rewrite PRES; [done| ].
+    eapply elem_of_dom; eauto. 
+    (* apply lookup_delete_Some in H0 as [??]. *)
+    (* apply mk_is_Some, elem_of_dom in H1. *)
+    (* rewrite DOM in H1. apply elem_of_set_seq in H1. *)
+    (* assert ((k <? m) = (k <? m + 1) \/ k = m). *)
+    (* { destruct (decide (k = m)); [tauto| ]. left. *)
+    (*   destruct (k <? m) eqn:LT. *)
+    (*   - rewrite (proj2 (PeanoNat.Nat.ltb_lt _ _)); [done | ]. *)
+    (*     apply PeanoNat.Nat.ltb_lt in LT. lia. *)
+    (*   - rewrite (proj2 (PeanoNat.Nat.ltb_ge _ _)); [done | ]. *)
+    (*     apply PeanoNat.Nat.ltb_ge in LT. lia. } *)
+    (* destruct H2; [| done]. rewrite H2. done. *)
+  Qed.
+
+  Lemma BMU_smap_extend `{invGS_gen HasNoLc Σ} τ m smap R B0
+    (PRES: forall i, i ∈ dom smap -> B0 (m + 1) i = B0 m i)
+    (FRESH_UNSET: B0 (m + 1) m = false):
+    ⊢ obls τ R (oGS := oGS) -∗ smap_repr (B0 m) m smap -∗
+      BMU ∅ 1 (
+        |==> (∃ s',
+             smap_repr (B0 (m + 1)) (m + 1) (<[m := s']> smap) ∗
+             ith_sig m s' ∗ obls τ (R ∪ {[s']}) (oGS := oGS) ∗
+             ⌜ s' ∉ R ⌝)) (oGS := oGS).
+    Proof using LEQUIV__l DISCR__l DISCR__d.
+      iIntros "OBLS SM".
+      iApply OU_BMU.
+      iDestruct (OU_create_sig with "OBLS") as "FOO".
+      iApply (OU_wand with "[-FOO]"); [| by iFrame].
+      iIntros "(%s' & SG & OBLS & %NEW)".
+      iApply BMU_intro.
+      rewrite /smap_repr. iDestruct "SM" as "(SM & %DOM & SIGS)". 
+      iMod (own_update with "SM") as "SM".
+      { apply auth_update_alloc. eapply (alloc_singleton_local_update _ m (to_agree s')).
+        2: done.
+        apply not_elem_of_dom. rewrite dom_fmap. rewrite DOM.
+        intros ?%elem_of_set_seq. lia. }
+      iModIntro. iDestruct "SM" as "[SM S']".
+      iExists s'.
+      rewrite -fmap_insert. iFrame. iSplit; [| done].
+      iSplitR.
+      { iPureIntro. rewrite dom_insert_L.
+        rewrite set_seq_add_L. rewrite -DOM. set_solver. }
+      iApply (smap_sgns_extend with "[$]"); try done.
+      rewrite FRESH_UNSET. iFrame.
+    Qed.
+      
+  (*   Lemma BMU_smap_restore τ s m smap *)
+  (*     (DOM : dom smap = set_seq 0 (B `min` (m + 2))) *)
+  (*     (IN : smap !! m = Some s) *)
+  (*     (lm : sigO (λ i : nat, i < LIM)) *)
+  (*     (LVL : lvl2nat lm = m): *)
+  (*       ⊢ *)
+  (* obls τ ∅ (oGS := oGS) -∗ *)
+  (* ([∗ map] k↦y ∈ delete m smap, ∃ l0 : sigO (λ i : nat, i < LIM), *)
+  (*                                         sgn y l0 (Some (k <? m)) (oGS := oGS) ∗ *)
+  (*                                         ⌜lvl2nat l0 = k⌝) -∗ *)
+  (* (sgn s lm (Some true) (oGS := oGS)) -∗ *)
+  (* own eofin_smap (● ((to_agree <$> smap): gmap _ _)) -∗ *)
+  (* BMU (⊤ ∖ ↑nroot.@"eofin") 1 *)
+  (*   (⌜B ≤ m + 2⌝ ∗ obls τ ∅ (oGS := oGS) ∗ smap_repr_eo (B `min` (m + 2)) (m + 1) smap *)
+  (*    ∨ (|==> ⌜m + 2 < B⌝ ∗ *)
+  (*         (∃ (s' : SignalId) (lm': EOLevel B), *)
+  (*            smap_repr_eo (B `min` (m + 3)) (m + 1) (<[m + 2:=s']> smap) ∗ *)
+  (*            ith_sig (m + 2) s' ∗ obls τ {[s']} (oGS := oGS) ∗ *)
+  (*            ⌜lvl2nat lm' = (m + 2)%nat⌝))) (oGS := oGS). *)
+  (*   Proof using. *)
+  (*     iIntros "OBLS SIGS SIG SM". *)
+  (*     destruct (Nat.le_gt_cases B (m + 2)). *)
+  (*     { rewrite PeanoNat.Nat.min_l in DOM; [| done].  *)
+  (*       iApply BMU_intro. iLeft. iFrame. *)
+  (*       iSplitR; [done| ]. iSplitR. *)
+  (*       { iPureIntro. rewrite PeanoNat.Nat.min_l; auto. } *)
+  (*       iApply (restore_map with "[$] [$]"); eauto. *)
+  (*       rewrite DOM. f_equal. symmetry. by apply Nat.min_l. } *)
+      
+  (*     iApply OU_BMU. *)
+  (*     assert {lm' : EOLevel B | lvl2nat lm' = m + 2} as [lm' LVL']. *)
+  (*     { set (lm' := exist _ (m + 2) H0: EOLevel B). *)
+  (*       exists lm'. done. } *)
+  (*     iDestruct (OU_create_sig with "OBLS") as "FOO". *)
+  (*     iApply (OU_wand with "[-FOO]"); [| by iFrame]. *)
+  (*     iIntros "(%s' & SG & OBLS & %NEW)". rewrite union_empty_l_L. *)
+  (*     iApply BMU_intro. iRight. iSplitR; [done| ]. *)
+  (*     rewrite PeanoNat.Nat.min_r in DOM; [| lia]. *)
+  (*     iMod (own_update with "SM") as "SM". *)
+  (*     { apply auth_update_alloc. eapply (alloc_singleton_local_update _ (m + 2) (to_agree s')). *)
+  (*       2: done.  *)
+  (*       apply not_elem_of_dom. rewrite dom_fmap. rewrite DOM. *)
+  (*       intros ?%elem_of_set_seq. lia. } *)
+  (*     iModIntro. iDestruct "SM" as "[SM S']". *)
+  (*     iExists s', lm'.  *)
+  (*     iSplitL "SIGS SG SIG SM". *)
+  (*     2: { iFrame. eauto. } *)
+  (*     rewrite PeanoNat.Nat.min_r; [| lia]. rewrite /smap_repr_eo. *)
+  (*     rewrite -fmap_insert. iFrame. iSplitR. *)
+  (*     { iPureIntro. rewrite dom_insert_L DOM. *)
+  (*       apply set_eq. intros ?. rewrite elem_of_union elem_of_singleton. *)
+  (*       rewrite !elem_of_set_seq. lia. } *)
+  (*     rewrite big_sepM_insert_delete. iSplitL "SG". *)
+  (*     { iExists _. rewrite (proj2 (PeanoNat.Nat.ltb_ge _ _)); [ | lia]. *)
+  (*       iFrame. iPureIntro. *)
+  (*       Unshelve. *)
+  (*       2: { assert (m + 2 < LIM) by lia.  *)
+  (*            esplit. apply H1. } *)
+  (*       done. } *)
+  (*     rewrite (delete_notin _ (m + 2)). *)
+  (*     2: { apply not_elem_of_dom. rewrite DOM. intros ?%elem_of_set_seq. lia. } *)
+  (*     iApply (restore_map with "[$] [$]"); eauto. *)
+  (*     rewrite DOM. f_equal. symmetry. lia. *)
+  (*   Qed. *)
+
+    Lemma ith_sig_expect i sw m τ π π__e smap R d B
+      (PH_EXP: phase_le π__e π)
+      (GE: m <= i)
+      (UNSETi: B i = false):
+      ⊢ ep sw π__e d (oGS := oGS) -∗ th_phase_ge τ π (oGS := oGS) -∗
+         smap_repr B m smap -∗ ith_sig i sw -∗
+         obls τ R (oGS := oGS) -∗ sgns_level_gt R (L i) (oGS := oGS) -∗ 
+         OU (∃ π', cp π' d (oGS := oGS) ∗ smap_repr B m smap ∗ th_phase_ge τ π' (oGS := oGS) ∗ obls τ R (oGS := oGS) ∗ ⌜ phase_le π π' /\ phase_le π__e π' ⌝) (oGS := oGS).
+    Proof using LEQUIV__l DISCR__l.
+      iIntros "#EP PH SR #SW OBLS #OBLS_LT". 
+      iDestruct (ith_sig_in with "[$] [$]") as "%ITH".
+      iDestruct (smap_repr_split with "SW [$]") as "[SGw SR]".
+      rewrite {1}/ex_ith_sig. rewrite UNSETi. 
+      iDestruct (expect_sig_upd with "EP [$] [$] [$] [$]") as "OU"; [done| ..].
+      iApply (OU_wand with "[-OU]"); [| done].
+      iIntros "(%π' & CP1 & SIGW & OBLS & PH & [%PH_LE' %PH_LE''])".
+      iExists _. iFrame. iSplitL; [| done].
+      iApply "SR". rewrite /ex_ith_sig. by rewrite UNSETi.
+    Qed.
+
+    Lemma smap_expose_dom B m smap:
+      ⊢ smap_repr B m smap -∗ ⌜ dom smap = set_seq 0 m ⌝.
+    Proof using. by iIntros "(?&?&?)". Qed.
+
+End SignalMap.
+
 Section EoFin.
   Context (B: nat).
   Let LIM := B + 1. 
@@ -33,7 +341,7 @@ Section EoFin.
   Let OM := ObligationsModel.
 
   Let EOLevelOfe := BNOfe LIM. 
-  Let EODegreeOfe := BNOfe NUM_DEG. 
+  Let EODegreeOfe := BNOfe NUM_DEG.
 
   Context `{EM: ExecutionModel heap_lang M}. 
   Context `{hGS: @heapGS Σ _ EM}.
@@ -59,13 +367,15 @@ Section EoFin.
 
   Class EoFinPreG Σ := {
       eofin_threads_PreG :> inG Σ (excl_authR natO);
-      eofin_sigs :> inG Σ (authUR (gmapUR nat (agreeR SignalId)));
+      eofin_sigs :> SigMapPreG Σ;
+        (* inG Σ (authUR (gmapUR nat (agreeR SignalId))); *)                 
   }.
   
   Class EoFinG Σ := {
       eofin_PreG :> EoFinPreG Σ;
       eofin_even: gname; eofin_odd: gname;
-      eofin_smap: gname;
+      (* eofin_smap: gname; *)
+      eofin_sm :> SigMapG Σ;
   }.
 
   Definition lvl2nat {X} (l: EOLevel X) := bn2nat _ l. 
@@ -137,213 +447,58 @@ Section EoFin.
 
   End ThreadResources.
 
-  Definition ex_ith_sig (n i: nat) (s: SignalId): iProp Σ :=
-    ∃ l, sgn s l (Some $ Nat.ltb i n) (oGS := oGS) ∗ ⌜ lvl2nat l = i ⌝. 
-  
-  Definition smap_repr' {PRE: EoFinPreG Σ} γ K n (smap: gmap nat SignalId): iProp Σ :=
-    own γ (● (to_agree <$> smap: gmapUR nat (agreeR SignalId))) ∗
-    ⌜ dom smap = set_seq 0 K ⌝ ∗
-    ([∗ map] i ↦ s ∈ smap, ex_ith_sig n i s).
-
   Section Threads.
     Context `{EoFinG Σ}.
-
-    Definition smap_repr := smap_repr' eofin_smap. 
     
     Definition threads_auth n: iProp Σ := 
       thread_auth eofin_even (if Nat.even n then n else n + 1) ∗
-      thread_auth eofin_odd (if Nat.odd n then n else n + 1). 
+      thread_auth eofin_odd (if Nat.odd n then n else n + 1).
+
+    Definition B__eo (i: nat): EOLevel LIM :=
+      match (le_lt_dec LIM i) with
+      | left GE => ith_bn LIM 0 ltac:(lia)                                      
+      | right LT => ith_bn LIM i LT
+      end.
+
+    Definition smap_repr_eo n := smap_repr B__eo (flip Nat.ltb n) (oGS := oGS). 
 
     Definition eofin_inv_inner l: iProp Σ :=
       ∃ (n: nat) (smap: gmap nat SignalId), 
-          l ↦ #n ∗ threads_auth n ∗ smap_repr (min B (n + 2)) n smap.
+          l ↦ #n ∗ threads_auth n ∗ smap_repr_eo n (min B (n + 2)) smap.
 
     Definition eofin_inv l: iProp Σ :=
       inv (nroot .@ "eofin") (eofin_inv_inner l).
 
-    Definition ith_sig (i: nat) (s: SignalId): iProp Σ :=
-      own eofin_smap (◯ {[ i := to_agree s ]}).
-
-    Definition ith_sig_in i s K n (smap: gmap nat SignalId):
-      ⊢ ith_sig i s -∗ smap_repr K n smap -∗ ⌜ smap !! i = Some s ⌝.
-    Proof.
-      iIntros "S (SM & ? & ?)". iCombine "SM S" as "SM".
-      iDestruct (own_valid with "SM") as %V.
-      apply auth_both_valid_discrete in V as [V ?].
-      apply singleton_included_l in V. destruct V as (x & ITH & LE).
-      iPureIntro.
-      rewrite Some_included_total in LE.
-      destruct (to_agree_uninj x) as [y X].
-      { eapply lookup_valid_Some; eauto. done. }
-      rewrite -X in LE. apply to_agree_included in LE.
-      rewrite -X in ITH.
-
-      eapply leibniz_equiv.       
-      rewrite lookup_fmap in ITH.
-      rewrite -LE in ITH.
-
-      apply fmap_Some_equiv in ITH as (?&?&?).
-      rewrite H1. apply to_agree_inj in H2. by rewrite H2.
-    Qed.
-
-    Definition ith_sig_sgn i s K n (smap: gmap nat SignalId):
-      ⊢ ith_sig i s -∗ smap_repr K n smap -∗ ∃ l, sgn s l None (oGS := oGS) ∗ ⌜ lvl2nat l = i ⌝. 
-    Proof.
-      iIntros "S SR".
-      iDestruct (ith_sig_in with "[$] [$]") as "%ITH". 
-      iDestruct "SR" as "(SM & % & ?)".
-      iDestruct (big_sepM_lookup with "[$]") as "ITH"; eauto.
-      rewrite /ex_ith_sig. iDestruct "ITH" as "(%l & SG & %LVL)".
-      iExists _. iSplitL; [| done].
-      by iDestruct (sgn_get_ex with "[$]") as "[??]". 
-    Qed.
-
-    Lemma smap_repr_split K n smap i s:
-      ⊢ ith_sig i s -∗ smap_repr K n smap -∗
-         ex_ith_sig n i s ∗ (ex_ith_sig n i s -∗ smap_repr K n smap).
-    Proof using.
-      iIntros "#ITH SR".
-      iDestruct (ith_sig_in with "[$] [$]") as "%ITH".
-      rewrite /smap_repr /smap_repr'. iDestruct "SR" as "(SM & % & SR)".
-      rewrite {2 5}(map_split smap i) ITH /=.
-      rewrite !big_sepM_union.
-      2: apply map_disjoint_singleton_l_2; by apply lookup_delete.
-      iDestruct "SR" as "[S SR]". rewrite big_sepM_singleton.
-      iFrame. iIntros. iFrame. done.
-    Qed.
-
-    (* TODO: use bupd in definition of OU *)
-    Lemma smap_create_ep i K n smap π π__cp τ
-      (PH_LE: phase_le π__cp π)
-      (LT: i < K):
-      ⊢ smap_repr K n smap -∗ 
-         cp π__cp d2 (oGS := oGS) -∗
-         th_phase_ge τ π (oGS := oGS) -∗
-         |==> OU (∃ s, ith_sig i s ∗
-             ep s π__cp d1 (oGS := oGS) ∗ smap_repr K n smap ∗
-            th_phase_ge τ π (oGS := oGS)) (oGS := oGS).
-    Proof using.
-      iIntros "SR CP PH".
-      rewrite /smap_repr /smap_repr'. iDestruct "SR" as "(AUTH & %DOM & SIGS)".
-      assert (i ∈ dom smap) as [s ITH]%elem_of_dom.
-      { rewrite DOM. apply elem_of_set_seq. lia. }
-      rewrite {2 5}(map_split smap i) ITH /=.
-      setoid_rewrite big_sepM_union.
-      2, 3: apply map_disjoint_singleton_l_2; by apply lookup_delete.
-      iDestruct "SIGS" as "[SIG SIGS]". setoid_rewrite big_sepM_singleton.
-      rewrite {1}/ex_ith_sig. iDestruct "SIG" as "(%l & SIG & %LVLi)".
-      iDestruct (create_ep_upd with "CP [$] [PH]") as "OU".
-      { apply (ith_bn_lt _ 1). lia. }
-      { done. }
-      { done. }
-      iMod (own_update with "AUTH") as "X". 
-      { apply auth_update_dfrac_alloc. 
-        2: { apply singleton_included_l with (i := i).
-             rewrite lookup_fmap ITH. eexists. split; [| reflexivity].
-             simpl. reflexivity. }
-        apply _. }
-      iApply (OU_wand with "[-OU]"); [| by iFrame].
-      iIntros "(EP & SIG & PH)".
-      iDestruct "X" as "[? ITH]". 
-      iExists _. iFrame. iSplitR; [done| ].
-      iExists _. by iFrame.
-    Qed.
-
-    Lemma restore_map (smap: gmap nat SignalId) (s : SignalId) (m : nat) lm
-      (DOM: dom smap = set_seq 0 (B `min` (m + 2)))
-      (IN: smap !! m = Some s)
-      (LVL: lvl2nat lm = m)
-      :
-      ⊢ (([∗ map] k↦y ∈ delete m smap,
-           ∃ l0, sgn y l0 (Some (k <? m)) (oGS := oGS) ∗ ⌜lvl2nat l0 = k⌝) -∗
-          sgn s lm (Some true) (oGS := oGS)-∗
-          [∗ map] i↦s0 ∈ smap,
-           ∃ l0, sgn s0 l0 (Some (i <? m + 1)) (oGS := oGS) ∗ ⌜ lvl2nat l0 = i⌝)%I.
-    Proof using.
-      iIntros "SIGS SG".
-      rewrite (big_sepM_delete _ smap); eauto.
-      iSplitL "SG".
-      { iExists _. rewrite (proj2 (Nat.ltb_lt _ _)); [| lia].
-        iFrame. done. }
-      iApply (big_sepM_impl with "[$]"). iModIntro.
-      iIntros (???) "(%&?&?)". iExists _. iFrame.
-      apply lookup_delete_Some in H0 as [??].
-      apply mk_is_Some, elem_of_dom in H1.
-      rewrite DOM in H1. apply elem_of_set_seq in H1.
-      assert ((k <? m) = (k <? m + 1) \/ k = m).
-      { destruct (decide (k = m)); [tauto| ]. left.
-        destruct (k <? m) eqn:LT.
-        - rewrite (proj2 (PeanoNat.Nat.ltb_lt _ _)); [done | ].
-          apply PeanoNat.Nat.ltb_lt in LT. lia.
-        - rewrite (proj2 (PeanoNat.Nat.ltb_ge _ _)); [done | ].
-          apply PeanoNat.Nat.ltb_ge in LT. lia. }
-      destruct H2; [| done]. rewrite H2. done.
-    Qed.
-
-    Lemma BMU_smap_restore τ s m smap
-      (DOM : dom smap = set_seq 0 (B `min` (m + 2)))
-      (IN : smap !! m = Some s)
-      (lm : sigO (λ i : nat, i < LIM))
-      (LVL : lvl2nat lm = m):
-        ⊢
-  obls τ ∅ (oGS := oGS) -∗
-  ([∗ map] k↦y ∈ delete m smap, ∃ l0 : sigO (λ i : nat, i < LIM),
-                                          sgn y l0 (Some (k <? m)) (oGS := oGS) ∗
-                                          ⌜lvl2nat l0 = k⌝) -∗
-  (sgn s lm (Some true) (oGS := oGS)) -∗
-  own eofin_smap (● ((to_agree <$> smap): gmap _ _)) -∗
-  BMU (⊤ ∖ ↑nroot.@"eofin") 1
-    (⌜B ≤ m + 2⌝ ∗ obls τ ∅ (oGS := oGS) ∗ smap_repr (B `min` (m + 2)) (m + 1) smap
-     ∨ (|==> ⌜m + 2 < B⌝ ∗
-          (∃ (s' : SignalId) (lm': EOLevel B),
-             smap_repr (B `min` (m + 3)) (m + 1) (<[m + 2:=s']> smap) ∗
-             ith_sig (m + 2) s' ∗ obls τ {[s']} (oGS := oGS) ∗
-             ⌜lvl2nat lm' = (m + 2)%nat⌝))) (oGS := oGS).
-    Proof using.
-      iIntros "OBLS SIGS SIG SM".
-      destruct (Nat.le_gt_cases B (m + 2)).
-      { rewrite PeanoNat.Nat.min_l in DOM; [| done]. 
-        iApply BMU_intro. iLeft. iFrame.
-        iSplitR; [done| ]. iSplitR.
-        { iPureIntro. rewrite PeanoNat.Nat.min_l; auto. }
-        iApply (restore_map with "[$] [$]"); eauto.
-        rewrite DOM. f_equal. symmetry. by apply Nat.min_l. }
-      
-      iApply OU_BMU.
-      assert {lm' : EOLevel B | lvl2nat lm' = m + 2} as [lm' LVL'].
-      { set (lm' := exist _ (m + 2) H0: EOLevel B).
-        exists lm'. done. }
-      iDestruct (OU_create_sig with "OBLS") as "FOO".
-      iApply (OU_wand with "[-FOO]"); [| by iFrame].
-      iIntros "(%s' & SG & OBLS & %NEW)". rewrite union_empty_l_L.
-      iApply BMU_intro. iRight. iSplitR; [done| ].
-      rewrite PeanoNat.Nat.min_r in DOM; [| lia].
-      iMod (own_update with "SM") as "SM".
-      { apply auth_update_alloc. eapply (alloc_singleton_local_update _ (m + 2) (to_agree s')).
-        2: done. 
-        apply not_elem_of_dom. rewrite dom_fmap. rewrite DOM.
-        intros ?%elem_of_set_seq. lia. }
-      iModIntro. iDestruct "SM" as "[SM S']".
-      iExists s', lm'. 
-      iSplitL "SIGS SG SIG SM".
-      2: { iFrame. eauto. }
-      rewrite PeanoNat.Nat.min_r; [| lia]. rewrite /smap_repr.
-      rewrite -fmap_insert. iFrame. iSplitR.
-      { iPureIntro. rewrite dom_insert_L DOM.
-        apply set_eq. intros ?. rewrite elem_of_union elem_of_singleton.
-        rewrite !elem_of_set_seq. lia. }
-      rewrite big_sepM_insert_delete. iSplitL "SG".
-      { iExists _. rewrite (proj2 (PeanoNat.Nat.ltb_ge _ _)); [ | lia].
-        iFrame. iPureIntro.
-        Unshelve.
-        2: { assert (m + 2 < LIM) by lia. 
-             esplit. apply H1. }
-        done. }
-      rewrite (delete_notin _ (m + 2)).
-      2: { apply not_elem_of_dom. rewrite DOM. intros ?%elem_of_set_seq. lia. }
-      iApply (restore_map with "[$] [$]"); eauto.
-      rewrite DOM. f_equal. symmetry. lia.
-    Qed.
+    (* Lemma restore_map (smap: gmap nat SignalId) (s : SignalId) (m : nat) lm *)
+    (*   (DOM: dom smap = set_seq 0 (B `min` (m + 2))) *)
+    (*   (IN: smap !! m = Some s) *)
+    (*   (LVL: lvl2nat lm = m) *)
+    (*   : *)
+    (*   ⊢ (([∗ map] k↦y ∈ delete m smap, *)
+    (*        ∃ l0, sgn y l0 (Some (k <? m)) (oGS := oGS) ∗ ⌜lvl2nat l0 = k⌝) -∗ *)
+    (*       sgn s lm (Some true) (oGS := oGS)-∗ *)
+    (*       [∗ map] i↦s0 ∈ smap, *)
+    (*        ∃ l0, sgn s0 l0 (Some (i <? m + 1)) (oGS := oGS) ∗ ⌜ lvl2nat l0 = i⌝)%I. *)
+    (* Proof using. *)
+    (*   iIntros "SIGS SG". *)
+    (*   rewrite (big_sepM_delete _ smap); eauto. *)
+    (*   iSplitL "SG". *)
+    (*   { iExists _. rewrite (proj2 (Nat.ltb_lt _ _)); [| lia]. *)
+    (*     iFrame. done. } *)
+    (*   iApply (big_sepM_impl with "[$]"). iModIntro. *)
+    (*   iIntros (???) "(%&?&?)". iExists _. iFrame. *)
+    (*   apply lookup_delete_Some in H0 as [??]. *)
+    (*   apply mk_is_Some, elem_of_dom in H1. *)
+    (*   rewrite DOM in H1. apply elem_of_set_seq in H1. *)
+    (*   assert ((k <? m) = (k <? m + 1) \/ k = m). *)
+    (*   { destruct (decide (k = m)); [tauto| ]. left. *)
+    (*     destruct (k <? m) eqn:LT. *)
+    (*     - rewrite (proj2 (PeanoNat.Nat.ltb_lt _ _)); [done | ]. *)
+    (*       apply PeanoNat.Nat.ltb_lt in LT. lia. *)
+    (*     - rewrite (proj2 (PeanoNat.Nat.ltb_ge _ _)); [done | ]. *)
+    (*       apply PeanoNat.Nat.ltb_ge in LT. lia. } *)
+    (*   destruct H2; [| done]. rewrite H2. done. *)
+    (* Qed. *)
 
     (* TODO: generalize, move *)
     Lemma lvl_lt_equiv (l1 l2: EOLevel LIM):
@@ -357,32 +512,6 @@ Section EoFin.
       - intros ?. split; [lia| ]. intros ?. inversion H1. subst. lia.
     Qed.
     
-    Lemma ith_sig_expect i sw m τ π π__e N smap s
-      (PH_EXP: phase_le π__e π)
-      (GE: m <= i):
-      ⊢ ep sw π__e d1 (oGS := oGS) -∗ th_phase_ge τ π (oGS := oGS) -∗
-         smap_repr N m smap -∗ ith_sig i sw -∗
-         ith_sig (i + 1) s -∗ obls τ {[ s ]} (oGS := oGS) -∗
-         OU (∃ π', cp π' d1 (oGS := oGS) ∗ smap_repr N m smap ∗ th_phase_ge τ π' (oGS := oGS) ∗ obls τ {[ s ]} (oGS := oGS) ∗ ⌜ phase_le π π' /\ phase_le π__e π' ⌝) (oGS := oGS).
-    Proof using.
-      iIntros "#EP PH SR #SW #S OBLS". 
-      iDestruct (ith_sig_in with "[$] [$]") as "%ITH".
-      iDestruct (ith_sig_sgn with "S [$]") as "#OWN".
-      iDestruct (smap_repr_split with "SW [$]") as "[SGw SR]".
-      rewrite {1}/ex_ith_sig. rewrite (proj2 (Nat.ltb_ge _ _)); [| done].
-      iDestruct "SGw" as "(%lw & SGw & %LW)".
-      iDestruct (expect_sig_upd with "EP [$] [$] [] [$]") as "OU"; [done| ..].
-      { rewrite /sgns_level_gt. rewrite big_sepS_singleton.
-        iDestruct "OWN" as "(%lo & SGo & %LO)".
-        iExists _. iFrame "SGo". iPureIntro.
-        apply lvl_lt_equiv. rewrite /lvl2nat in LW, LO. lia. }
-      iApply (OU_wand with "[-OU]"); [| done].
-      iIntros "(%π' & CP1 & SIGW & OBLS & PH & [%PH_LE' %PH_LE''])".
-      iExists _. iFrame. iSplitL; [| done].
-      iApply "SR". iExists _.
-      rewrite (proj2 (Nat.ltb_ge _ _)); [| done]. by iFrame.
-    Qed.
-
     Record ThreadResource (th_res: nat -> iProp Σ) (cond: nat -> bool) := {
         tr_agree (n1 n2: nat): threads_auth n1-∗ th_res n2 -∗
                               ⌜ n2 = if (cond n1) then n1 else (n1 + 1)%nat ⌝;
@@ -445,32 +574,42 @@ Section EoFin.
         { econstructor. done. }
         iNext. iIntros "L".
         
-        iDestruct (ith_sig_in with "[$] [$]") as %IN.
-        iDestruct "SR" as "(SM & %DOM & SIGS)".
+        (* iDestruct (ith_sig_in with "[$] [$]") as %IN. *)
+        (* iDestruct "SR" as "(SM & %DOM & SIGS)". *)
         
-        iDestruct (big_sepM_delete with "SIGS") as "[SG SIGS]"; eauto.
-        iDestruct "SG" as (lm) "(SG & %LVL)".
-        rewrite Nat.ltb_irrefl. 
+        (* iDestruct (big_sepM_delete with "SIGS") as "[SG SIGS]"; eauto. *)
+        (* iDestruct "SG" as (lm) "(SG & %LVL)". *)
+        iDestruct (smap_expose_dom with "[$]") as "%SM_DOM". 
+        rewrite /smap_repr_eo. 
+        
+        iPoseProof (smap_repr_split_upd B__eo _ (flip Nat.ltb (m + 1)) with "[$] [$]") as "[SG SR_CLOS]".
+        { intros ?. rewrite SM_DOM elem_of_set_seq. simpl.
+          intros NEQ [? [??]%Nat.min_glb_lt_iff].
+          assert (j < m \/ j = m + 1) as [? | ->] by lia.
+          - rewrite !(proj2 (PeanoNat.Nat.ltb_lt _ _)); lia.
+          - rewrite !(proj2 (PeanoNat.Nat.ltb_ge _ _)); lia. }        
         
         MU_by_BMU. iApply OU_BMU.
         iDestruct (OU_set_sig with "OB [SG]") as "OU".
         { apply elem_of_singleton. reflexivity. }
-        { by iFrame. }
+        { rewrite /ex_ith_sig. simpl. rewrite Nat.ltb_irrefl. iFrame. }
         iApply (OU_wand with "[-OU]"); [| done]. iIntros "(SIG & OBLS)".
-        rewrite (subseteq_empty_difference_L {[ s ]}); [| done].        
+        rewrite (subseteq_empty_difference_L {[ s ]}); [| done].
         
-        iPoseProof (BMU_smap_restore with "OBLS [$] [$] [$]") as "BMU"; eauto.
+        (* iPoseProof (BMU_smap_restore with "OBLS [$] [$] [$]") as "BMU"; eauto. *)
+        iSpecialize ("SR_CLOS" with "[SIG]").
+        { rewrite /ex_ith_sig. simpl.
+          rewrite !(proj2 (PeanoNat.Nat.ltb_lt _ _)); [iFrame | lia]. }
         iApply (BMU_lower _ 1); [lia| ].
-        iApply (BMU_wand with "[-BMU] [$]"). iIntros "COND".
-        
+        Unshelve. 2: by apply _.
+        (* iApply (BMU_wand with "[-BMU] [$]"). iIntros "COND". *)
+        iApply BMU_intro. 
         iDestruct (cp_mul_take with "CPS") as "[CPS CP]".
         iSplitR "CP".
         2: { do 2 iExists _. iFrame. done. }
         iApply wp_value.
         
         iMod (tr_update with "[$] TH") as "[AUTH TH]"; eauto. 
-
-        (* rewrite E in H0. *)
 
         destruct (Nat.le_gt_cases B (m + 2)). 
         + iDestruct "COND" as "[COND | CC]".
@@ -737,7 +876,7 @@ Section EoFin.
       apply elem_of_dom in DOMm as [? DOMm]. by rewrite DOMm.
     Qed. 
 
-    (* TODO: parametrize smap_repr with the lower bound *)
+    (* TODO: parametrize smap_repr_eo with the lower bound *)
     Lemma alloc_inv l (* (i: nat) *) τ
       (* (i := 0) *)
       :
@@ -758,7 +897,7 @@ Section EoFin.
       
       set (m := min B 2).
       iAssert (BMU ⊤ 2 
-                 (|==> ∃ γ smap, smap_repr' γ m 0 smap ∗
+                 (|==> ∃ γ smap, smap_repr_eo' γ m 0 smap ∗
                                  (* let sigs := map_img smap in *)
                                  let sigs := sigs_block smap 0 m in
                                  obls τ (list_to_set sigs) (oGS := oGS) ∗
@@ -844,7 +983,7 @@ Section EoFin.
 
           iSplitR "OB".
           2: { iFrame. iPureIntro; constructor. }
-          rewrite /smap_repr'. iFrame.
+          rewrite /smap_repr_eo'. iFrame.
           iSplitR.
           { subst smap0. iPureIntro. 
             subst m. (* subst i. *)
